## Consider the sequence of steps to solve the equation: 2(x – 4) + 6x = 9x – 10 Given = 2(x – 4) + 6x = 9x – 10 Step 1 = 2x – 8 +

Question

Consider the sequence of steps to solve the equation: 2(x – 4) + 6x = 9x – 10

Given = 2(x – 4) + 6x = 9x – 10

Step 1 = 2x – 8 + 6x = 9x – 10

Step 2 = 2x + 6x – 8 = 9x – 10

Step 3 8x – 8 = 9x – 10

Step 4 = 8x – 8x – 8 = 9x – 8x – 10

Step 5 = 0 – 8 = x – 10

Step 6 = -8 = x – 10

Step 7 = -8 + 10 = x – 10 + 10

Step 8 = 2 = x + 0

Step 9 = 2 = x

Which step in solving this equation is justified by the Distributive Property?

in progress
0

Math
4 weeks
2021-09-16T18:51:35+00:00
2021-09-16T18:51:35+00:00 1 Answer
0
## Answers ( )

step 1 because the 2 is multiplied by the (x-4)